src/ptt.v
@@ -4,7 +4,8 @@ Require syntax.
 
 Section Ptt.
 
-Local Instance havePrecondition : config.Precondition := {| config.flagPrecondition := config.Yes |}.
+Local Instance havePrecondition : config.Precondition :=
+  {| config.flagPrecondition := config.Yes |}.
 Context `{configReflection : config.Reflection}.
 Context `{configBinaryProdType : config.BinaryProdType}.
 Context `{configProdEta : config.ProdEta}.
